---
layout: post
title:  "Berry phase"
math: true
date:   2018-08-09 22:37:04 -0500
categories: jekyll update
---
The physical quantity is the Chern number, which represents the Hall conductivity, 

$$ n = \frac{1}{2\pi} \int \Omega_{xy} dk^2, $$

where the definition of Berry curvature is

$$
\Omega_{xy} = i<\partial _x u|\partial _y u> -  i<\partial _y u|\partial _x u>.
$$

In area with boundary C, Stoke's theorem gives

$$
\int \Omega_{xy} dk^2 = \oint_C A_k  \cdot dk.
$$

The connection is, $$ A _k= i <u | \partial_k u> $$.
Since $$ u_{k+G }(r) = e^{i\phi_G(k)}e^{-iGr}  u_k(r) $$,
the Berry connnection is not periodic,

$$ A_{k+G} = A_k - \partial_k \phi_G$$


The chern number is, due to phase uncertainty is $2\pi Z$. 

$$
n = \frac{1}{2\pi} ( \theta_x(1)-\theta_x(0)  + \theta_y(0)-\theta_y(1)) \in Z
$$

The relation to phase connections are,

$$
\theta_x (x)= \phi_y(x,0), \theta_y  = \phi_x(0,y)
$$

Note the factor 
$$
e^{-iGr}
$$
does not effect the Berry curvature. 



### Polarization

$$
\dot x = \frac{\partial \varepsilon}{\partial k } - \Omega_{kt}
$$

Therefore,


$$
k a = 2\pi \cdot i/N , \delta k  = \frac{2\pi}{L}
$$

$$
j = \frac{|e|}{Na} \sum_k \Omega_{kt} = \frac{e}{2\pi} \int dk\Omega_{kt} =  \frac{e}{2\pi} \int dk (\frac{\partial A_t}{\partial k } - \frac{\partial A_k}{\partial t } )
$$


If $A_t (k + G) = A_t (k)$ , then 

$$
\int dk\Omega_{kt}   =-\frac{\partial }{\partial t }  \int dk A_k
$$

In this 1D system, the condition means keeping the periodic boundary condition: phase $\phi_k$ does not depend on $t$. 
$$
u_{k+G }(r;t) = e^{-iGr}  u_k(r;t) e^{i\phi_G}
$$

we have the polarization definition 

$$
P = \frac{e}{2\pi} \int dk A_k
$$

$$
j = - \frac{\partial}{\partial t} P
$$

$$
P(T)- P(0) = - \int j  \cdot dt =-\frac{e}{2\pi} \int dkdt\cdot \Omega_{kt} =  -e c
$$

For 2D, the phase factor has two component, 

$$
\left [
\begin{array}{cc}
\phi_{x}(k_x,k_y) \\
\phi_{y} (k_x,k_y)
\end{array}
\right]
$$

On the boundary it is 

$$
\left [
\begin{array}{cc}
\phi_{x}(0,k_y) \\
\phi_{y} (k_x,0)
\end{array}
\right]
$$

A proper definition for polarzation in 1D along $x$ direction requires 

$$
\phi_{x} = \phi_{x} (k_x,\cancel {k_y})  , \ \ \ \ \ \forall k_y \in [-\pi,\pi]
$$

in the continum condition. For the boundary with $k_x =0$, that is 

$$
\phi_{x} (0,\cancel {k_y} ) = \text{constant} \equiv \phi_0
$$

This is almost a Berry phase, excep the begin and end wavefunction are different. 

$$
u_{G} (r)= e^{i\phi_0}e^{-iGr}u_{0}(r)
$$

### TB model

The tight bind basis

$$
c^\dagger_k = \frac{1}{\sqrt N} \sum \exp^{ikR_i} c_i^\dagger
$$

Or 

$$
\phi_k^\alpha(r) = \frac{1}{\sqrt N } \sum \exp(ikR_i) \delta (r - R_i -d_\alpha)
$$

The Bloch wavefunction

$$
\psi_k(r) = \sum \eta_k^\alpha \phi_k^\alpha(r) =   \frac{1}{\sqrt N } \sum \eta_k^\alpha \exp(ikR_i) \delta (r - R_i -d_\alpha)
$$

which satisfies

$$
\psi_k(r+a) = e^{ika} \psi_k(r)
$$

The periodic part is 
$$
u_k(r) = e(-ikr) \psi_k(r) =\frac{1}{\sqrt N } \sum \eta_k^\alpha \exp[-ik(r-R_i)] \delta (r - R_i -d_\alpha)
$$

Or 

$$
u_k(r) =\frac{1}{\sqrt N } \sum \eta_k^\alpha \exp[-ik d_\alpha] \delta (r - R_i -d_\alpha)
$$

The priodic contraint is 

$$
\psi_{k+G } (r)   = e^{i\phi_k} \psi_k(r)
$$

Or 

$$
u_{k+G }(r) = e^{i\phi_k}e^{-iGr}  u_k(r)
$$

Since $\eta_{k+G} = e^{i\phi_G(k)} \eta_k$,

$$
L.H.S = e^{i\phi_G}\frac{1}{\sqrt N } \sum \eta_{k}^\alpha \exp[-i(k+G) d_\alpha] \delta (r - R_i -d_\alpha)
$$

while

$$
R.H.S = e^{i\phi_G}\frac{1}{\sqrt N } \sum \eta_k^\alpha \exp[-ik d_\alpha - iGr]  \delta (r - R_i -d_\alpha)
$$

Or 

$$
R.H.S =  e^{i\phi_G}\frac{1}{\sqrt N } \sum \eta_k^\alpha \exp[-i(k+G) d_\alpha]  \delta (r - R_i -d_\alpha) = L.H.S
$$

And the phase $\phi_G(k)$ is from $\eta_k$ . 



### The Berry phase or Zak phase

Since

$$
u_{k+G }(r) = e^{i\phi_G}e^{-iGr}  u_k(r)
$$

the Zak phase along one direction in k space is 

$$
\Phi = - i \log(<u_0|u_1> <u_1|u_2> \dots <u_{n-1}|  u_n>)
$$

or 

$$
\Phi = - i \log(<u_0|u_1> <u_1|u_2> \dots <u_{n-1}|  e^{i\phi_0}e^{-iGr} |u_0>)
$$

Using 

$$
u_k(r) =\frac{1}{\sqrt N } \sum \eta_k^\alpha \exp[-ik d_\alpha] \delta (r - R_i -d_\alpha) = \frac{1}{\sqrt N } \sum \tilde \eta_k^\alpha \delta (r - R_i -d_\alpha)
$$

where 

$$
\tilde \eta ^\alpha_k  =  \eta^\alpha _ke^{-ikd_\alpha}
$$

We have 

$$
<u_0|u_1> = \sum \eta_0^{\alpha*} \eta_1^\alpha \exp[-i(k_1-k_0) d_\alpha] = <\tilde \eta_0 | \tilde \eta_1>
$$

$$
\dots
$$

$$
<u_{n-1}|u_n> =\sum \eta_{n-1}^{\alpha*} \eta_n^\alpha  \exp[-i(k_{n}-k_{n-1} ) d_\alpha] = < \tilde \eta_{n-1}| \tilde \eta_n >
$$

or 

$$
\color{blue} {<u_{n-1}|u_n> =\sum \eta_{n-1}^{\alpha*} \eta_0^\alpha  e^{i\phi_0} \exp[-i(k_{0}-k_{n-1} + G) d_\alpha] = < \tilde \eta_{n-1}|  \Lambda_G|\tilde \eta_0 > + \phi_0}
$$

and 

$$k_n - G = k_0$$

$$
\eta_n e^{-i\phi_0} = \eta_0
$$

which needs to be kept for any t ($k_y$). In numerical diagonalization, $\phi_0$ may change with t ($k_y$). So just use the one with $\eta_0$. 

Therefore 

$$
\Phi = - i \log(<\tilde \eta_0|\tilde \eta_1> <\tilde \eta_1|\tilde \eta_2> \dots <\tilde \eta_{n-1}|\tilde \eta_n>)
$$


Note 

$$
\tilde \eta _k  =   \Lambda _k\eta _k
$$

with 

$$
\Lambda_k = 
\left(
\begin{array}{ccccc}
e^{-ikd_0}                                    \\
& e^{-ikd_1}            &   & 0\\
&               & \dots                \\
& 0 &   & e^{-ikd_{n-1}}            \\
&               &   &   & e^{-ikd_n}
\end{array}
\right)
$$

$$
\Phi = - i \log(< \eta_0|\Lambda_0^\dagger \Lambda_1| \eta_1> <  \eta_1| \Lambda_1^\dagger \Lambda_2|  \eta_2> \dots < \eta_{n-1}|\Lambda_{n-1}^\dagger \Lambda_n|  \eta_n>)
$$

$$
\color{red}{\Phi = - i \log(< \eta_0|\Lambda_0^\dagger \Lambda_1| \eta_1> <  \eta_1| \Lambda_1^\dagger \Lambda_2|  \eta_2> \dots < \eta_{n-1}|\Lambda_{n-1}^\dagger \Lambda_n |  \eta_0>) + \phi_0}
$$

Or 

$$
\Phi = - i \log[Tr(\Lambda_0^\dagger \Lambda_1| \eta_1> <  \eta_1| \Lambda_1^\dagger \Lambda_2|  \eta_2> \dots < \eta_{n-1}|\Lambda_{n-1}^\dagger \Lambda_n|  \eta_n><\eta_0|)]
$$

$$
\color{red}{\Phi = - i \log[Tr(\Lambda_0^\dagger \Lambda_1| \eta_1> <  \eta_1| \Lambda_1^\dagger \Lambda_2|  \eta_2> \dots < \eta_{n-1}|\Lambda_{n-1}^\dagger \Lambda_n|\eta_0><\eta_0|)] + \phi_0}
$$



For 2D case, $\phi_0$ is contant for any $k_y$; thus often ignored in calcuating 

$$
c = \frac{1}{2\pi} [\Phi (k_y = \pi) - \Phi (k_y = -\pi)]
$$

In case $d_\alpha = d_0$ 

$$
\Phi = - i \log(< \eta_0|  \eta_1> <  \eta_1|  \eta_2> \dots < \eta_{n-1}| \eta_0>)
$$

Comments

1. $\phi_0$ has uncertainty of $2\pi$. It is chosen as along as the smooth condition is satisified. In 1D, this phase factor can always be $\phi_0= 0$. 

2. The fact, that $\Lambda$ matrix effects the Berry phase $\Phi$, means that, the distribution of charge within the unit cell gives rise to a contribution to the charge polarization. *Example:* 
$$
\eta_i =
\left(
\begin{array}{c}
1,0 \dots
\end{array}
\right)
$$

$$
\Phi = -i \log[\exp(i(k_0 - k_n)d_1)] = (k_0-k_n) d_1 = -Gd_1
$$





[1](https://journals.aps.org/rmp/pdf/10.1103/RevModPhys.82.1959)

[2](https://journals.aps.org/prl/pdf/10.1103/PhysRevLett.62.2747)

